First version of 2 Ctor proofs

Examples/CtorStore/CtorStore.sol
@@ -1,0 +1,10 @@
+// SPDX-License-Identifier: UNLICENSED
+pragma solidity ^0.8.23;
+
+contract CtorStore {
+    uint256 private stored;
+
+    constructor(uint256 x) payable {
+        stored = x;
+    }
+}
